semantics.v
@@ -1,0 +1,78 @@
+Require Export proof_outlines.
+
+Definition state := var -> option Z.
+
+Inductive value :=
+| VInt(z: Z)
+| VBool(b: bool)
+.
+
+Inductive evaluates_to(S: state): term -> value -> Prop :=
+| Val_evaluates_to z:
+  evaluates_to S (Val z) (VInt z)
+| Var_evaluates_to x z:
+  S x = Some z ->
+  evaluates_to S (Var x) (VInt z)
+| Add_evaluates_to t1 t2 z1 z2:
+  evaluates_to S t1 (VInt z1) ->
+  evaluates_to S t2 (VInt z2) ->
+  evaluates_to S (BinOp Add t1 t2) (VInt (z1 + z2))
+| Sub_evaluates_to t1 t2 z1 z2:
+  evaluates_to S t1 (VInt z1) ->
+  evaluates_to S t2 (VInt z2) ->
+  evaluates_to S (BinOp Sub t1 t2) (VInt (z1 - z2))
+| Eq_evaluates_to_true t1 t2 v:
+  evaluates_to S t1 v ->
+  evaluates_to S t2 v ->
+  evaluates_to S (BinOp Eq t1 t2) (VBool true)
+| Eq_evaluates_to_false t1 t2 v1 v2:
+  evaluates_to S t1 v1 ->
+  evaluates_to S t2 v2 ->
+  v1 <> v2 ->
+  evaluates_to S (BinOp Eq t1 t2) (VBool false)
+| Not_evaluates_to t b:
+  evaluates_to S t (VBool b) ->
+  evaluates_to S (Not t) (VBool (if b then false else true))
+.
+
+Definition update(x: var)(z: Z)(S: state): state :=
+  fun y => if string_dec x y then Some z else S y.
+
+Inductive terminates_in: state -> stmt -> state -> Prop :=
+| Assert_terminates_in S P j:
+  evaluates_to S P (VBool true) ->
+  terminates_in S (Assert P j) S
+| Assign_terminates_in S x t z:
+  evaluates_to S t (VInt z) ->
+  terminates_in S (Assign x t) (update x z S)
+| Pass_terminates_in S:
+  terminates_in S Pass S
+| Seq_terminates_in S s1 S' s2 S'':
+  terminates_in S s1 S' ->
+  terminates_in S' s2 S'' ->
+  terminates_in S (s1 ;; s2) S''
+| If_terminates_in S C b s1 s2 S':
+  evaluates_to S C (VBool b) ->
+  terminates_in S (if b then s1 else s2) S' ->
+  terminates_in S (If C s1 s2) S'
+| While_terminates_in S C s S':
+  terminates_in S (If C (s ;; While C s) Pass) S' ->
+  terminates_in S (While C s) S'
+.
+
+CoInductive diverges: state -> stmt -> Prop :=
+| Seq_diverges1 S s1 s2:
+  diverges S s1 ->
+  diverges S (s1 ;; s2)
+| Seq_diverges2 S s1 S' s2:
+  terminates_in S s1 S' ->
+  diverges S' s2 ->
+  diverges S (s1 ;; s2)
+| If_diverges S C s1 s2 b:
+  evaluates_to S C (VBool b) ->
+  diverges S (if b then s1 else s2) ->
+  diverges S (If C s1 s2)
+| While_diverges S C s:
+  diverges S (If C (s ;; While C s) Pass) ->
+  diverges S (While C s)
+.
