soundness.v
@@ -1,0 +1,257 @@
+Require Export semantics proof_checker.
+
+Inductive is_safe(S: state)(s: stmt): Prop :=
+| terminates_is_safe S':
+  terminates_in S s S' ->
+  is_safe S s
+| diverges_is_safe:
+  diverges S s ->
+  is_safe S s.
+
+Definition env := list var.
+
+Inductive type := TInt | TBool.
+
+Definition type_eq_dec(t1 t2: type): {t1 = t2} + {t1 <> t2}.
+decide equality.
+Defined.
+
+Definition type_eqb(t1 t2: type): bool :=
+  if type_eq_dec t1 t2 then true else false.
+
+Section TypeChecking.
+
+Context (E: env).
+
+Fixpoint type_of(t: term): option type :=
+  match t with
+    Val z => Some TInt
+  | Var x => if in_dec string_dec x E then Some TInt else None
+  | BinOp (Add|Sub) t1 t2 =>
+    match type_of t1, type_of t2 with
+      Some TInt, Some TInt => Some TInt
+    | _, _ => None
+    end
+  | BinOp Eq t1 t2 =>
+    match type_of t1, type_of t2 with
+      Some TInt, Some TInt => Some TInt
+    | _, _ => None
+    end
+  | BinOp And t1 t2 =>
+    match type_of t1, type_of t2 with
+      Some TBool, Some TBool => Some TBool
+    | _, _ => None
+    end
+  | Not t =>
+    match type_of t with
+      Some TBool => Some TBool
+    | _ => None
+    end
+  end.
+
+End TypeChecking.
+
+Fixpoint stmt_is_well_typed(E: env)(s: stmt): option env :=
+  match s with
+    Assert P j =>
+    match type_of E P with
+      Some TBool => Some E
+    | _ => None
+    end
+  | Assign x t =>
+    match type_of E t with
+      Some TInt => Some (x::E)
+    | _ => None
+    end
+  | Pass => Some E
+  | If C s1 s2 =>
+    match type_of E C with
+      Some TBool =>
+      match stmt_is_well_typed E s1 with
+        Some E1 =>
+        match stmt_is_well_typed E s2 with
+          Some E2 =>
+          Some E
+        | _ => None
+        end
+      | _ => None
+      end
+    | _ => None
+    end
+  | While C s =>
+    match type_of E C with
+      Some TBool =>
+      match stmt_is_well_typed E s with
+        Some _ => Some E
+      | _ => None
+      end
+    | _ => None
+    end
+  | s1 ;; s2 =>
+    match stmt_is_well_typed E s1 with
+      Some E => stmt_is_well_typed E s2
+    | None => None
+    end
+  end.
+
+Inductive poly_evaluates_to(S: var -> option Z): list (Z * term) -> Z -> Prop :=
+| empty_poly_evaluates_to:
+  poly_evaluates_to S [] 0
+| nonempty_poly_evaluates_to z t vt p vp:
+  evaluates_to S t (VInt vt) ->
+  poly_evaluates_to S p vp ->
+  poly_evaluates_to S ((z, t)::p) (z * vt + vp)
+.
+
+Lemma poly_scale_soundness S p vp z:
+  poly_evaluates_to S p vp ->
+  poly_evaluates_to S (poly_scale z p) (z * vp).
+Proof.
+  revert p vp.
+  induction p; intros.
+  - inversion H; clear H; subst.
+    rewrite Z.mul_0_r.
+    constructor.
+  - inversion H; clear H; subst.
+    simpl.
+    rewrite Z.mul_add_distr_l.
+    rewrite Z.mul_assoc.
+    constructor; auto.
+Qed.
+
+Lemma evaluates_to_unique S t v1:
+  evaluates_to S t v1 ->
+  forall v2,
+  evaluates_to S t v2 ->
+  v1 = v2.
+Proof.
+  induction 1; intros.
+  - inversion H; clear H; subst; reflexivity.
+  - inversion H0; clear H0; subst. congruence.
+  - inversion H1; clear H1; subst.
+    apply IHevaluates_to1 in H4.
+    apply IHevaluates_to2 in H6.
+    congruence.
+  - inversion H1; clear H1; subst.
+    apply IHevaluates_to1 in H4.
+    apply IHevaluates_to2 in H6.
+    congruence.
+  - inversion H1; clear H1; subst.
+    + apply IHevaluates_to1 in H4.
+      apply IHevaluates_to2 in H6.
+      congruence.
+    + apply IHevaluates_to1 in H4.
+      apply IHevaluates_to2 in H5.
+      subst.
+      congruence.
+  - inversion H2; clear H2; subst.
+    + apply IHevaluates_to1 in H5.
+      apply IHevaluates_to2 in H7.
+      congruence.
+    + reflexivity.
+  - inversion H0; clear H0; subst.
+    apply IHevaluates_to in H2.
+    injection H2; clear H2; intros; subst.
+    reflexivity.
+Qed.
+
+Lemma poly_add_term_soundness S z t vt p vp:
+  evaluates_to S t (VInt vt) ->
+  poly_evaluates_to S p vp ->
+  poly_evaluates_to S (poly_add_term z t p) (z * vt + vp).
+Proof.
+  revert p vp.
+  induction p; intros.
+  - inversion H0; clear H0; subst.
+    simpl.
+    constructor; auto.
+    constructor.
+  - inversion H0; clear H0; subst.
+    simpl.
+    destruct (term_eq_dec t t0).
+    + subst.
+      destruct (Z.eq_dec (z + z0) 0).
+      * rewrite e.
+        rewrite Z.eqb_refl.
+        apply evaluates_to_unique with (1:=H) in H3.
+        injection H3; clear H3; intros; subst.
+        rewrite Z.add_assoc.
+        rewrite <- Z.mul_add_distr_r.
+        rewrite e.
+        rewrite Z.mul_0_l.
+        rewrite Z.add_0_l.
+        assumption.
+      * 
+
+Lemma poly_add_soundness S p1 z1 p2 z2:
+  poly_evaluates_to S p1 z1 ->
+  poly_evaluates_to S p2 z2 ->
+  poly_evaluates_to S (poly_add p1 p2) (z1 + z2).
+
+Lemma poly_subtract_soundness S p1 z1 p2 z2:
+  poly_evaluates_to S p1 z1 ->
+  poly_evaluates_to S p2 z2 ->
+  poly_evaluates_to S (poly_subtract p1 p2) (z1 - z2).
+  
+
+Lemma poly_of_soundness E t:
+  type_of E t = Some TInt ->
+  forall S,
+  Forall (fun x => S x <> None) E ->
+  exists z,
+  poly_evaluates_to S (poly_of t) z /\
+  evaluates_to S t (VInt z).
+
+Lemma Z_tautology_checker_soundness E C:
+  type_of E C = Some TBool ->
+  is_Z_tautology C = true ->
+  forall S,
+  Forall (fun x => S x <> None) E ->
+  evaluates_to S C (VBool true).
+Proof.
+  
+Lemma conjunct_entailment_checker_soundness E Hs C j:
+  Forall (fun H => type_of E H = Some TBool) Hs ->
+  type_of E C = Some TBool ->
+  is_valid_conjunct_entailment Hs C j = true ->
+  forall S,
+  Forall (fun x => S x <> None) E ->
+  Forall (fun H => evaluates_to S H (VBool true)) Hs ->
+  evaluates_to S C (VBool true).
+Proof.
+
+Lemma entailment_checker_soundness E P P' j:
+  type_of E P = Some TBool ->
+  type_of E P' = Some TBool ->
+  is_valid_entailment P P' j = true ->
+  forall S,
+  Forall (fun x => S x <> None) E ->
+  evaluates_to S P (VBool true) ->
+  evaluates_to S P' (VBool true).
+Proof.
+  
+
+Lemma soundness_lemma:
+  forall E P j s,
+  stmt_is_well_typed E (Assert P j ;; s) <> None ->
+  is_valid_proof_outline (Assert P j ;; s) = true ->
+  forall S,
+  Forall (fun x => S x <> None) E ->
+  evaluates_to S P (VBool true) ->
+  (forall S', ~ terminates_in S s S') ->
+  diverges S s.
+Proof.
+  cofix Hcofix.
+  intros.
+  destruct s; simpl in H0; try discriminate.
+  - destruct s1; simpl in H0.
+    + apply Seq_diverges2 with (S':=S).
+      * constructor.
+
+Theorem soundness E P j s:
+  stmt_is_well_typed E (Assert P j ;; s) <> None ->
+  is_valid_proof_outline (Assert P j ;; s) = true ->
+  forall S,
+  Forall (fun x => S x <> None) E ->
+  evaluates_to S P (VBool true) ->
+  is_safe S s.
